update poly1305 api

tests/tests-openssl/poly1305-test.c
@@ -9,9 +9,9 @@
 #include <stdbool.h>
 #include <time.h>
 
-#include "Hacl_Poly1305_32.h"
-#include "Hacl_Poly1305_128.h"
-#include "Hacl_Poly1305_256.h"
+#include "Hacl_MAC_Poly1305.h"
+#include "Hacl_MAC_Poly1305_Simd128.h"
+#include "Hacl_MAC_Poly1305_Simd256.h"
 
 #include "test_helpers.h"
 #include "poly1305_vectors.h"
@@ -50,15 +50,15 @@ bool print_result(uint8_t* comp, uint8_t* exp) {
 bool print_test(int in_len, uint8_t* in, uint8_t* key, uint8_t* exp){
   uint8_t comp[16] = {0};
 
-  Hacl_Poly1305_32_poly1305_mac(comp,in_len,in,key);
+  Hacl_MAC_Poly1305_poly1305_mac(comp,in_len,in,key);
   printf("Poly1305 (32-bit) Result:\n");
   bool ok = print_result(comp, exp);
 
-  Hacl_Poly1305_128_poly1305_mac(comp,in_len,in,key);
+  Hacl_MAC_Poly1305_Simd128_poly1305_mac(comp,in_len,in,key);
   printf("Poly1305 (128-bit) Result:\n");
   ok = ok && print_result(comp, exp);
 
-  Hacl_Poly1305_256_poly1305_mac(comp,in_len,in,key);
+  Hacl_MAC_Poly1305_Simd256_poly1305_mac(comp,in_len,in,key);
   printf("Poly1305 (256-bit) Result:\n");
   ok = ok && print_result(comp, exp);
 
@@ -88,13 +88,13 @@ int main() {
   memset(plain,'P',SIZE);
   memset(key,'K',16);
   for (int j = 0; j < ROUNDS; j++) {
-    Hacl_Poly1305_32_poly1305_mac(plain,SIZE,plain,key);
+    Hacl_MAC_Poly1305_poly1305_mac(plain,SIZE,plain,key);
   }
 
   t1 = clock();
   a = cpucycles_begin();
   for (int j = 0; j < ROUNDS; j++) {
-    Hacl_Poly1305_32_poly1305_mac(tag,SIZE,plain,key);
+    Hacl_MAC_Poly1305_poly1305_mac(tag,SIZE,plain,key);
     res ^= tag[0] ^ tag[15];
   }
   b = cpucycles_end();
@@ -106,13 +106,13 @@ int main() {
   memset(plain,'P',SIZE);
   memset(key,'K',16);
   for (int j = 0; j < ROUNDS; j++) {
-    Hacl_Poly1305_128_poly1305_mac(plain,SIZE,plain,key);
+    Hacl_MAC_Poly1305_Simd128_poly1305_mac(plain,SIZE,plain,key);
   }
 
   t1 = clock();
   a = cpucycles_begin();
   for (int j = 0; j < ROUNDS; j++) {
-    Hacl_Poly1305_128_poly1305_mac(tag,SIZE,plain,key);
+    Hacl_MAC_Poly1305_Simd128_poly1305_mac(tag,SIZE,plain,key);
     res ^= tag[0] ^ tag[15];
   }
   b = cpucycles_end();
@@ -124,13 +124,13 @@ int main() {
   memset(plain,'P',SIZE);
   memset(key,'K',16);
   for (int j = 0; j < ROUNDS; j++) {
-    Hacl_Poly1305_256_poly1305_mac(plain,SIZE,plain,key);
+    Hacl_MAC_Poly1305_Simd256_poly1305_mac(plain,SIZE,plain,key);
   }
 
   t1 = clock();
   a = cpucycles_begin();
   for (int j = 0; j < ROUNDS; j++) {
-    Hacl_Poly1305_256_poly1305_mac(tag,SIZE,plain,key);
+    Hacl_MAC_Poly1305_Simd256_poly1305_mac(tag,SIZE,plain,key);
     res ^= tag[0] ^ tag[15];
   }
   b = cpucycles_end();
