code/poly1305/Hacl.Poly1305_32.fsti
@@ -19,4 +19,4 @@ val poly1305_update: poly1305_update_st M32
 
 val poly1305_finish: poly1305_finish_st M32
 
-val poly1305_mac: poly1305_mac_st M32
+val mac: poly1305_mac_st M32
