dist/package-mozilla.sh
@@ -24,9 +24,9 @@ FILES=" \
   Hacl_IntTypes_Intrinsics_128 \
   Hacl_Krmllib \
   Hacl_Lib \
-  Hacl_Poly1305_128 \
-  Hacl_Poly1305_256 \
-  Hacl_Poly1305_32 \
+  Hacl_MAC_Poly1305_Simd128 \
+  Hacl_MAC_Poly1305_Simd256 \
+  Hacl_MAC_Poly1305 \
   Hacl_RSAPSS \
   Hacl_SHA2_Types \
   Hacl_Spec \
